Optimise use of tree composition
Signed-off-by: zeramorphic <zeramorphic@proton.me>

ConNF/Foa/Approximation/StructApprox.lean
@@ -22,10 +22,10 @@ abbrev StructApprox :=
 namespace StructApprox
 
 def Approximates {β : TypeIndex} (π₀ : StructApprox β) (π : StructPerm β) : Prop :=
-  ∀ A, (π₀ A).Approximates (Tree.ofBot <| Tree.comp A π)
+  ∀ A, (π₀ A).Approximates (π A)
 
 def ExactlyApproximates {β : TypeIndex} (π₀ : StructApprox β) (π : StructPerm β) : Prop :=
-  ∀ A, (π₀ A).ExactlyApproximates (Tree.ofBot <| Tree.comp A π)
+  ∀ A, (π₀ A).ExactlyApproximates (π A)
 
 variable {α : Λ} [BasePositions] [Phase2Assumptions α]
 
@@ -35,18 +35,12 @@ def Free {β : Iic α} (π₀ : StructApprox β) : Prop :=
 theorem Approximates.comp {β γ : TypeIndex} {π₀ : StructApprox β} {π : StructPerm β}
     (h : π₀.Approximates π) (A : Path β γ) :
     StructApprox.Approximates (π₀.comp A) (Tree.comp A π) :=
-  by
-  intro B
-  rw [Tree.comp_apply, Tree.comp_comp]
-  exact h _
+  fun B => h (A.comp B)
 
 theorem ExactlyApproximates.comp {β γ : TypeIndex} {π₀ : StructApprox β} {π : StructPerm β}
     (h : π₀.ExactlyApproximates π) (A : Path β γ) :
     StructApprox.ExactlyApproximates (π₀.comp A) (Tree.comp A π) :=
-  by
-  intro B
-  rw [Tree.comp_apply, Tree.comp_comp]
-  exact h _
+  fun B => h (A.comp B)
 
 /-!
 # Induction on support conditions
