ConNF/Foa/Action/StructAction.lean
@@ -46,34 +46,24 @@ theorem complete_apply (hφ : φ.Lawful) (B : ExtendedIndex β) :
 
 theorem smul_atom_eq {hφ : φ.Lawful} {π : StructPerm β} (hπ : (φ.complete hφ).ExactlyApproximates π)
     {a : Atom} {B : ExtendedIndex β} (ha : ((φ B).atomMap a).Dom) :
-    Tree.comp B π • a = ((φ B).atomMap a).get ha := by
-  have := (φ B).smul_atom_eq (hπ B) ha
-  rw [Tree.ofBot_smul] at this
-  exact this
+    π B • a = ((φ B).atomMap a).get ha :=
+  (φ B).smul_atom_eq (hπ B) ha
 
 theorem smul_toNearLitter_eq_of_precise {hφ : φ.Lawful} (hφp : φ.Precise) {π : StructPerm β}
     (hπ : (φ.complete hφ).ExactlyApproximates π) {L : Litter} {B : ExtendedIndex β}
     (hL : ((φ B).litterMap L).Dom)
-    (hπL : Tree.comp B π • L = (((φ B).litterMap L).get hL).1) :
-    Tree.comp B π • L.toNearLitter = ((φ B).litterMap L).get hL := by
-  have := (φ B).smul_toNearLitter_eq_of_preciseAt (hπ B) hL (hφp B hL) ?_
-  · rw [Tree.ofBot_smul] at this
-    exact this
-  · rw [Tree.ofBot_smul]
-    exact hπL
+    (hπL : π B • L = (((φ B).litterMap L).get hL).1) :
+    π B • L.toNearLitter = ((φ B).litterMap L).get hL :=
+  (φ B).smul_toNearLitter_eq_of_preciseAt (hπ B) hL (hφp B hL) hπL
 
 theorem smul_nearLitter_eq_of_precise {hφ : φ.Lawful} (hφp : φ.Precise) {π : StructPerm β}
     (hπ : (φ.complete hφ).ExactlyApproximates π) {N : NearLitter} {B : ExtendedIndex β}
     (hN : ((φ B).litterMap N.1).Dom)
-    (hπL : Tree.comp B π • N.1 = (((φ B).litterMap N.1).get hN).1) :
-    ((Tree.comp B π • N : NearLitter) : Set Atom) =
+    (hπL : π B • N.1 = (((φ B).litterMap N.1).get hN).1) :
+    ((π B • N : NearLitter) : Set Atom) =
       (((φ B).litterMap N.1).get hN : Set Atom) ∆
-        (Tree.comp B π • litterSet N.1 ∆ N) := by
-  have := (φ B).smul_nearLitter_eq_of_preciseAt (hπ B) hN (hφp B hN) ?_
-  · rw [Tree.ofBot_smul] at this
-    exact this
-  · rw [Tree.ofBot_smul]
-    exact hπL
+        (Tree.comp B π • litterSet N.1 ∆ N) :=
+  (φ B).smul_nearLitter_eq_of_preciseAt (hπ B) hN (hφp B hN) hπL
 
 end Precise
 
